\subsection{Implementation}
\label{subsec:implementation}

Before proceeding with the discussion about the results, we report here the code implementation used to perform the dynamic analysis of the structure due to the moving load.

Using \texttt{MATLAB}, the code is the following:

\begin{lstlisting}[language=Matlab]

    load_position = @(t) ...
        (t <= t1) .*                             (1/2 * a * t.^2) + ...
        (t > t1 & t <= (t1 + t2)) .*             (1/2 * a * t1^2 + v * (t - t1)) + ...
        (t > (t1 + t2) & t <= (t1 + t2 + t3)) .* (1/2 * a * t1^2 + v * t2 + v * (t - (t2 + t1)) - 1/2 * a * (t - (t1 + t2)).^2) + ...
        (t > (t1 + t2 + t3)) .*                  (1/2 * a * t1^2 + v * t2 + v * t3 - 1/2 * a * t3.^2);

    Q_func = @(t) Phi' * compute_nodal_load(load_position(t), xy, idb, -9.81 * 40e3);

    initial_conditions = [zeros(length(Q_func(0)), 1) zeros(length(Q_func(0)), 1)];
    initial_conditions = [zeros(length(Q_func(0)), 1) K_FF_modal \ Q_func(0)];

    [t, z] = ode45( ...
        @(t, z) EquationOfMotion(t, z, M_FF_modal, C_FF_modal, K_FF_modal, Q_func), ...
        [0 max(t_vet)], ...
        initial_conditions, ...
        odeset('RelTol', 1e-6, 'AbsTol', 1e-6));

    X_moving_load = Phi * z(:, size(Phi, 2)+1:end)';

    %% Functions

    function [z_dot] = EquationOfMotion(t, z, M_FF_modal, C_FF_modal, K_FF_modal, Q_func)

        N_considered_modes = size(K_FF_modal, 1);

        q_dot = z(1:N_considered_modes, 1);
        q = z(N_considered_modes + (1:N_considered_modes), 1);

        % M * x_dot_dot + C * x_dot + K * x = F(t) -> Modal coordinates -> q
        q_dot_dot = M_FF_modal \ (Q_func(t) - C_FF_modal * q_dot - K_FF_modal * q);

        z_dot(1:N_considered_modes, 1) = q_dot_dot;
        z_dot(N_considered_modes + (1:N_considered_modes), 1) = q_dot;

    end


    function F_nodal = compute_nodal_load(load_position, xy, idb, F0)
    % Strictly related to our case at hand, nodes D to A.

        F_nodal = zeros(71, 1);

        if (load_position + xy(7, 1) < xy(8, 1))

            L = xy(8, 1) - xy(7, 1);
            xi = (load_position) / L;

            N1 = 1 - xi;
            N2 = xi;

            F_nodal(idb(7, 2)) = F0 * N1;
            F_nodal(idb(8, 2)) = F0 * N2;

        else

            L = xy(9, 1) - xy(8, 1);
            xi = (load_position - (xy(8, 1) - xy(7, 1))) / L;

            N1 = 1 - xi;
            N2 = xi;

            F_nodal(idb(8, 2)) = F0 * N1;
            F_nodal(idb(9, 2)) = F0 * N2;

        end

end

\end{lstlisting}
